new/code/github_com/sanjit_bhat/pav/ktcore.v
@@ -45,7 +45,7 @@ Definition CheckBlame : go_string := "github.com/sanjit-bhat/pav/ktcore.CheckBla
 
 (* CheckBlame prevents bad parties from giving bad [Blame] codes.
 
-   go: ktcore.go:32:6 *)
+   go: ktcore.go:34:6 *)
 Definition CheckBlameⁱᵐᵖˡ : val :=
   λ: "b" "allowed",
     exception_do (let: "err" := (mem.alloc (type.zero_val #boolT)) in
@@ -73,7 +73,7 @@ Definition VrfSig : go_type := structT [
 
 Definition VrfSigTag : val := #(W8 0).
 
-(* go: ktcore.go:40:6 *)
+(* go: ktcore.go:42:6 *)
 Definition SignVrfⁱᵐᵖˡ : val :=
   λ: "sk" "vrfPk",
     exception_do (let: "sig" := (mem.alloc (type.zero_val #sliceT)) in
@@ -98,7 +98,7 @@ Definition SignVrfⁱᵐᵖˡ : val :=
 
 Definition VerifyVrfSig : go_string := "github.com/sanjit-bhat/pav/ktcore.VerifyVrfSig"%go.
 
-(* go: ktcore.go:48:6 *)
+(* go: ktcore.go:50:6 *)
 Definition VerifyVrfSigⁱᵐᵖˡ : val :=
   λ: "pk" "vrfPk" "sig",
     exception_do (let: "err" := (mem.alloc (type.zero_val #boolT)) in
@@ -135,7 +135,7 @@ Definition LinkSig : go_type := structT [
 
 Definition LinkSigTag : val := #(W8 1).
 
-(* go: ktcore.go:54:6 *)
+(* go: ktcore.go:56:6 *)
 Definition SignLinkⁱᵐᵖˡ : val :=
   λ: "sk" "epoch" "link",
     exception_do (let: "sig" := (mem.alloc (type.zero_val #sliceT)) in
@@ -163,7 +163,7 @@ Definition SignLinkⁱᵐᵖˡ : val :=
 
 Definition VerifyLinkSig : go_string := "github.com/sanjit-bhat/pav/ktcore.VerifyLinkSig"%go.
 
-(* go: ktcore.go:62:6 *)
+(* go: ktcore.go:64:6 *)
 Definition VerifyLinkSigⁱᵐᵖˡ : val :=
   λ: "pk" "epoch" "link" "sig",
     exception_do (let: "err" := (mem.alloc (type.zero_val #boolT)) in
@@ -200,7 +200,7 @@ Definition MapLabel : go_type := structT [
 #[global] Typeclasses Opaque MapLabel.
 #[global] Opaque MapLabel.
 
-(* go: ktcore.go:68:6 *)
+(* go: ktcore.go:70:6 *)
 Definition ProveMapLabelⁱᵐᵖˡ : val :=
   λ: "sk" "uid" "ver",
     exception_do (let: "proof" := (mem.alloc (type.zero_val #sliceT)) in
@@ -226,7 +226,7 @@ Definition ProveMapLabelⁱᵐᵖˡ : val :=
 
 Definition EvalMapLabel : go_string := "github.com/sanjit-bhat/pav/ktcore.EvalMapLabel"%go.
 
-(* go: ktcore.go:74:6 *)
+(* go: ktcore.go:76:6 *)
 Definition EvalMapLabelⁱᵐᵖˡ : val :=
   λ: "sk" "uid" "ver",
     exception_do (let: "label" := (mem.alloc (type.zero_val #sliceT)) in
@@ -250,7 +250,7 @@ Definition EvalMapLabelⁱᵐᵖˡ : val :=
 
 Definition CheckMapLabel : go_string := "github.com/sanjit-bhat/pav/ktcore.CheckMapLabel"%go.
 
-(* go: ktcore.go:80:6 *)
+(* go: ktcore.go:82:6 *)
 Definition CheckMapLabelⁱᵐᵖˡ : val :=
   λ: "pk" "uid" "ver" "proof",
     exception_do (let: "err" := (mem.alloc (type.zero_val #boolT)) in
@@ -280,7 +280,7 @@ Definition GetMapVal : go_string := "github.com/sanjit-bhat/pav/ktcore.GetMapVal
 
 Definition CommitOpenEncode : go_string := "github.com/sanjit-bhat/pav/ktcore.CommitOpenEncode"%go.
 
-(* go: ktcore.go:86:6 *)
+(* go: ktcore.go:88:6 *)
 Definition GetMapValⁱᵐᵖˡ : val :=
   λ: "pkOpen",
     exception_do (let: "val" := (mem.alloc (type.zero_val #sliceT)) in
@@ -298,7 +298,7 @@ Definition GetCommitRand : go_string := "github.com/sanjit-bhat/pav/ktcore.GetCo
 (* GetCommitRand computes the psuedo-random (wrt commitSecret) bits
    used in a mapVal commitment.
 
-   go: ktcore.go:93:6 *)
+   go: ktcore.go:95:6 *)
 Definition GetCommitRandⁱᵐᵖˡ : val :=
   λ: "commitSecret" "label",
     exception_do (let: "rand" := (mem.alloc (type.zero_val #sliceT)) in
